more repl_exp_val
remaining subgoal is to show that the machine state (i.e. environment
and store) matches the semantic state after running the exp, and this is
almost in the assumptions except the store is (probably) syneq rather
than equal.

compiler/correctness/replScript.sml
@@ -10,7 +10,7 @@ val good_contab_def = Define`
 val env_rs_def = Define`
   env_rs env rs c rd s bs =
     (rs.rbvars = MAP FST env) ∧
-    good_code_env c ∧
+    code_env_code c c bs.code ∧
     FDOM c ⊆ count rs.rnext_label ∧
     let Cenv = env_to_Cenv (cmap rs.contab) env in
     Cenv_bs c rd s Cenv rs.renv rs.rsz bs`
@@ -401,6 +401,13 @@ val compile_c_SUBMAP = store_thm("compile_c_SUBMAP",
   strip_tac >- rw[compile_def] >>
   strip_tac >- rw[compile_def])
 
+val code_env_code_append = store_thm("code_env_code_append",
+  ``∀c d code code'. code_env_code c d code ∧ ALL_DISTINCT (FILTER is_Label (code ++ code')) ⇒
+    code_env_code c d (code ++ code')``,
+  simp[code_env_code_def,FEVERY_DEF] >> rw[] >>
+  res_tac >> HINT_EXISTS_TAC >> simp[] >>
+  qexists_tac`bc0`>>simp[])
+
 val repl_exp_val = store_thm("repl_exp_val",
   ``∀cenv s c env exp s' v rd rs rs' bc0 bc bs bs'.
       exp_pred exp ∧
@@ -511,13 +518,64 @@ val repl_exp_val = store_thm("repl_exp_val",
   qmatch_assum_abbrev_tac`bc_next bs bs1` >>
   qspecl_then[`Cc`,`Cs`,`Cenv`,`Ce`,`(Cs',Rval Cv)`]mp_tac(CONJUNCT1 compile_val) >> simp[] >>
   disch_then(qspecl_then[`rd`,`SND cce`,`rs.renv`,`rs.rsz`,`bs1`,`bc0 ++ REVERSE (SND cce).out`,`REVERSE bc`,`bc0 ++ REVERSE (SND cce).out`]mp_tac) >>
+  `code_env_code Cc Cc (bc0 ++ REVERSE (SND cce).out)` by (
+    simp[Abbr`Cenv`,Abbr`Cs`,env_to_Cenv_MAP,LIST_TO_SET_MAP,GSYM IMAGE_COMPOSE,combinTheory.o_DEF,all_Clocs_v_to_Cv,Abbr`bs1`] >>
+    simp[code_env_code_def,FILTER_APPEND,ALL_DISTINCT_APPEND,Abbr`Cc`] >>
+    conj_tac >- (
+      match_mp_tac good_code_env_FUNION >>
+      fs[env_rs_def,code_env_code_def] >>
+      simp[DISJOINT_DEF,EXTENSION,MEM_GENLIST] >>
+      gen_tac >> spose_not_then strip_assume_tac >>
+      fsrw_tac[DNF_ss][SUBSET_DEF] >>
+      res_tac >> fsrw_tac[ARITH_ss][]) >>
+    conj_tac >- (
+      fsrw_tac[DNF_ss][EVERY_MAP,EVERY_FILTER,is_Label_rwt,MEM_FILTER,MEM_GENLIST,between_def] >>
+      fsrw_tac[DNF_ss][EVERY_MEM] >>
+      rw[] >> spose_not_then strip_assume_tac >> res_tac >> fsrw_tac[ARITH_ss][] ) >>
+    rfs[env_rs_def,code_env_code_def] >>
+    rfs[FEVERY_DEF] >>
+    gen_tac >>
+    Cases_on`x ∈ FDOM c`>>simp[FUNION_DEF] >- (
+      last_x_assum(qspec_then`x`mp_tac) >>
+      simp[] >> strip_tac >>
+      qexists_tac`cs` >>
+      Q.PAT_ABBREV_TAC`cp = compile X Y Z A B C` >>
+      qmatch_assum_abbrev_tac`cq.out = cc ++ cs.out` >>
+      `cp = cq` by (
+        map_every qunabbrev_tac[`cp`,`cq`] >>
+        match_mp_tac (CONJUNCT1 compile_c_SUBMAP) >>
+        simp[SUBMAP_FUNION] >>
+        fs[good_code_env_def,IN_FRANGE] >>
+        metis_tac[] ) >>
+      simp[] >> qexists_tac`bc0'` >> simp[] ) >>
+    strip_tac >>
+    first_x_assum(qspec_then`x`mp_tac) >>
+    simp[] >> strip_tac >>
+    qexists_tac`cs` >>
+    Q.PAT_ABBREV_TAC`cp = compile X Y Z A B C` >>
+    qmatch_assum_abbrev_tac`cq.out = cc ++ cs.out` >>
+    `cp = cq` by (
+      map_every qunabbrev_tac[`cp`,`cq`] >>
+      match_mp_tac (CONJUNCT1 compile_c_SUBMAP) >>
+      conj_tac >- (
+        rfs[good_code_env_def,IN_FRANGE] >>
+        metis_tac[] ) >>
+      match_mp_tac SUBMAP_FUNION >>
+      simp[IN_DISJOINT] >> disj2_tac >>
+      gen_tac >> spose_not_then strip_assume_tac >>
+      fsrw_tac[DNF_ss][EVERY_MEM,MEM_GENLIST,SUBSET_DEF] >>
+      res_tac >> fsrw_tac[ARITH_ss][] ) >>
+    simp[] >>
+    qexists_tac`bc0 ++ bc0'` >>
+    simp[FILTER_APPEND] >>
+    fs[EVERY_FILTER,is_Label_rwt,GSYM LEFT_FORALL_IMP_THM] >>
+    fsrw_tac[DNF_ss][EVERY_MEM] >>
+    rw[] >> res_tac >> fs[MEM_GENLIST] >>
+    DECIDE_TAC ) >>
   discharge_hyps >- (
     simp[Abbr`Cenv`,Abbr`Cs`,env_to_Cenv_MAP,LIST_TO_SET_MAP,GSYM IMAGE_COMPOSE,combinTheory.o_DEF,all_Clocs_v_to_Cv,Abbr`bs1`] >>
     conj_tac >- ( fsrw_tac[DNF_ss][SUBSET_DEF] >> PROVE_TAC[] ) >>
     conj_tac >- ( fsrw_tac[DNF_ss][SUBSET_DEF] >> PROVE_TAC[] ) >>
-    conj_tac >- (
-      simp[code_env_code_def,FILTER_APPEND,ALL_DISTINCT_APPEND,Abbr`Cc`] >>
-      cheat ) >>
     conj_tac >- (
       match_mp_tac SUBSET_TRANS >>
       HINT_EXISTS_TAC >>
@@ -578,19 +636,27 @@ val repl_exp_val = store_thm("repl_exp_val",
       qabbrev_tac`ct=rs.contab` >>
       PairCases_on`ct` >> fs[good_contab_def] >>
       qspecl_then[`cenv`,`s`,`env`,`exp`,`s',Rval v`]mp_tac (CONJUNCT1 evaluate_all_cns) >>
-      fs[good_cmap_def] >>
+      fs[good_cmap_def,closed_under_cenv_def] >>
       fs[SUBSET_DEF,MEM_MAP,EXISTS_PROD] >>
-
-      cheat ) >>
+      metis_tac[]) >>
     match_mp_tac (MP_CANON Cv_bv_ov) >>
     HINT_EXISTS_TAC >> simp[] ) >>
   conj_tac >- (
-    simp[Abbr`Cc`] >>
-    match_mp_tac good_code_env_FUNION >>
-    simp[DISJOINT_DEF,EXTENSION] >>
-    fs[SUBSET_DEF,MEM_GENLIST] >>
-    gen_tac >> spose_not_then strip_assume_tac >>
-    res_tac >> fsrw_tac[ARITH_ss][] ) >>
+    match_mp_tac code_env_code_append >>
+    rfs[Abbr`cce`] >>
+    simp[FILTER_APPEND,ALL_DISTINCT_APPEND,FILTER_REVERSE,ALL_DISTINCT_REVERSE] >>
+    simp[MEM_FILTER,is_Label_rwt,GSYM LEFT_FORALL_IMP_THM] >>
+    fsrw_tac[DNF_ss][EVERY_MAP,EVERY_FILTER,is_Label_rwt,MEM_GENLIST,between_def] >>
+    fsrw_tac[DNF_ss][EVERY_MEM] >>
+    rw[] >> spose_not_then strip_assume_tac >> res_tac >> fsrw_tac[ARITH_ss][] ) >>
+  conj_tac >- (
+    rfs[Abbr`Cc`] >>
+    fsrw_tac[DNF_ss][SUBSET_DEF,MEM_GENLIST] >>
+    rw[] >> res_tac >> DECIDE_TAC ) >>
+  match_mp_tac Cenv_bs
+  fs[Cenv_bs_def]
+  DB.find"Cenv_bs"
+  Cenv_bs
 
 set_trace"goalstack print goal at top"0
 
